cryptis/lib/dh.v
@@ -91,7 +91,7 @@ have exps_t': exps t' = [a].
   apply Permutation_singleton_r.
   rewrite /t' (_ : TExp g a = TExpN g [a]); last by rewrite /TExpN TMulN1.
   have atom_a : atomic [a] by rewrite /atomic; apply/Forall_singleton.
-  by rewrite (exps_TExpN' gNX atom_a (invs_canceled1 Nm_a)).
+  by rewrite (exps_TExpN' gNX atom_a (no_inv_singleton Nm_a)).
 (* /MOVE *)
 have a_t' : a ∈ exps t' by rewrite exps_t'; set_solver.
 iPoseProof (exp_pred_inv_same with "p_t") as "[#contra|H]" => //.
@@ -119,7 +119,7 @@ have atom_ab : atomic [a; b].
   by rewrite /atomic Forall_cons Forall_singleton; split.
 have exps_t : exps (TExpN g [a; b]) ≡ₚ [a; b].
   by rewrite (exps_TExpN' gXN atom_ab
-    (proj2 (invs_canceled2 Nm_a Nm_b) a_bV)).
+    (proj2 (no_inv2 Nm_a Nm_b) a_bV)).
 have a_t : a ∈ exps (TExpN g [a; b]) by rewrite exps_t; set_solver.
 have b_t : b ∈ exps (TExpN g [a; b]) by rewrite exps_t; set_solver.
 iPoseProof (exp_pred_exps a_t with "p") as "[dh_a _]".
@@ -158,7 +158,7 @@ rewrite public_TExp_iff //; do !iSplit => //.
   apply Permutation_singleton_r.
   rewrite (_ : TExp g a = TExpN g [a]); last by rewrite /TExpN TMulN1.
   have atom_a : atomic [a] by rewrite /atomic; apply/Forall_singleton.
-  by rewrite (exps_TExpN' gXN atom_a (invs_canceled1 Nm_a)).
+  by rewrite (exps_TExpN' gXN atom_a (no_inv_singleton Nm_a)).
 - iModIntro; iIntros "#p".
   by iApply False_public; last iApply "aP1".
 Qed.
