examples/iso_dh/proofs/base.v
@@ -354,7 +354,7 @@ rewrite (_ : TExp (TInt 0) a = TExpN (TInt 0) [a]); last by rewrite /TExpN TMulN
 rewrite exps_TExpN' //.
 - by case.
 - by rewrite /atomic; apply/Forall_singleton.
-- exact: (invs_canceled1 Nm).
+- exact: (no_inv_singleton Nm).
 Qed.
 
 Lemma public_dh_secret1 a b :
@@ -388,7 +388,7 @@ move=> Nm_a Nm_b; iIntros "%a_b %a_bV #pred_a #pred_b #p".
 have NInt : ¬ is_exp (TInt 0) by case.
 have atom_ab : atomic [a; b] by rewrite /atomic Forall_cons Forall_singleton; split.
 have ic_ab : forall x, x ∈ [a; b] -> TInv x ∉ [a; b]
-  by apply/(invs_canceled2 Nm_a Nm_b).
+  by apply/(no_inv2 Nm_a Nm_b).
 iPoseProof (public_minted with "p") as "m".
 iAssert (minted a ∧ minted b)%I as "[ma mb]".
   rewrite minted_TExpN //. iDestruct "m" as "[_ m]". rewrite /=.
